theory/JITState.thy
@@ -1,0 +1,50 @@
+theory JITState
+imports
+  Main
+  rBPFCommType rBPFSyntax rBPFSem
+  x64Syntax x64Semantics x64Assembler Proof1
+  JIT_def
+begin
+
+record JitProgram =
+page_size     :: usize
+pc_section    :: "usize list"
+text_section  :: "x64_bin"
+
+record jit_state =
+jit_result :: JitProgram 
+offset_in_text_section :: usize 
+jit_pc :: usize
+
+abbreviation "REG_SCRATCH::ireg \<equiv> R11"
+
+definition bpf_to_x64_reg:: "bpf_ireg \<Rightarrow> ireg" where
+  "bpf_to_x64_reg br = (
+  case br of
+  BR0 \<Rightarrow> RAX |
+  BR1 \<Rightarrow> RDI |
+  BR2 \<Rightarrow> RSI |
+  BR3 \<Rightarrow> RDX |
+  BR4 \<Rightarrow> RCX |
+  BR5 \<Rightarrow> R8  |
+  BR6 \<Rightarrow> RBX |
+  BR7 \<Rightarrow> R13 |
+  BR8 \<Rightarrow> R14 |
+  BR9 \<Rightarrow> R15 |
+  BR10 \<Rightarrow> RBP
+)"
+
+lemma bpf_to_x64_reg_corr2[simp]:" bpf_to_x64_reg r1 \<noteq> bpf_to_x64_reg r2  \<longrightarrow> r1 \<noteq> r2 "
+  apply(unfold bpf_to_x64_reg_def)
+  apply(cases r1; cases r2; simp)
+  done
+
+lemma bpf_to_x64_reg_corr[simp]:" r1 \<noteq> r2 \<longrightarrow> bpf_to_x64_reg r1 \<noteq> bpf_to_x64_reg r2 "
+  apply(unfold bpf_to_x64_reg_def)
+  apply(cases r1; cases r2; simp)
+  done
+
+definition update_pc_section_aux ::"usize list \<Rightarrow> nat \<Rightarrow> usize \<Rightarrow> usize list" where
+"update_pc_section_aux pc_sec pc x = list_update pc_sec pc x"
+
+end
